Complexitylib/Classes.lean
@@ -17,6 +17,7 @@ import Complexitylib.Classes.NP
 import Complexitylib.Classes.Randomized
 import Complexitylib.Classes.Randomized.GoodSeed
 import Complexitylib.Classes.Randomized.CircuitAmplification
+import Complexitylib.Classes.Randomized.PPoly
 import Complexitylib.Classes.Pairing
 import Complexitylib.Classes.FNP
 import Complexitylib.Classes.NP.Witness
